Unstable -- preparing to try new parse table representation

LL1/ParseTableGen.v
@@ -8,43 +8,160 @@ Require Import LL1.ParseTable.
 
 Import ListNotations.
 
-Definition prod_la_pair := (production * LaSet.t)%type.
-Definition prod_la_pair_wf (g : grammar) (p : prod_la_pair) :=
-  match p with
-  | ((x, gamma), laSet) => lookahead_set_for laSet x gamma g
-  end.
-Definition prod_la_pairs_wf (ps : list prod_la_pair) (g : grammar) :=
-  Forall (prod_la_pair_wf g) ps.
-
-Definition empty_pt := NtMap.empty (LaMap.t (list symbol)).
+Definition prod_la_pair := (production * lookahead)%type.
 
 Definition singletonLaMap la gamma :=
   LaMap.add la gamma (LaMap.empty (list symbol)).
-  
-Definition addEntry (x : nonterminal) (la : lookahead) (gamma : list symbol) (o : option parse_table) :=
+
+Definition empty_pt := NtMap.empty (LaMap.t (list symbol)).
+
+Definition pairs_wf ps g :=
+  forall x gamma la,
+    In ((x, gamma), la) ps <-> lookahead_for la x gamma g.
+
+Definition addEntry (p : prod_la_pair) o :=
   match o with
   | None => None
-  | Some tbl => 
-    match NtMap.find x tbl with
-    | None => Some (NtMap.add x (singletonLaMap la gamma) tbl)
-    | Some m =>
-      match LaMap.find la m with
-      | None => Some (NtMap.add x (LaMap.add la gamma m) tbl)
-      | Some gamma' =>
-        if list_eq_dec symbol_eq_dec gamma gamma' then Some tbl else None
+  | Some tbl =>
+    match p with
+    | ((x, gamma), la) =>
+      match NtMap.find x tbl with
+      | None => Some (NtMap.add x (singletonLaMap la gamma) tbl)
+      | Some m =>
+        match LaMap.find la m with
+        | None => Some (NtMap.add x (LaMap.add la gamma m) tbl)
+        | Some gamma' =>
+          if list_eq_dec symbol_eq_dec gamma gamma' then Some tbl else None
+        end
       end
     end
   end.
 
-Definition addEntries (p : prod_la_pair) (o : option parse_table) :=
-  match p with
-  | ((x, gamma), laSet) =>
-    fold_right (fun la o => addEntry x la gamma o) o (LaSet.elements laSet)
-  end.
+Definition mkParseTable (ps : list prod_la_pair) :=
+  fold_right addEntry (Some empty_pt) ps.
 
-Definition mkParseTable (productions_with_la_sets : list prod_la_pair) :=
-  fold_right addEntries (Some empty_pt) productions_with_la_sets.
+Definition tbl_correct_wrt_pairs tbl ps :=
+  forall x gamma la,
+    pt_lookup x la tbl = Some gamma <-> In ((x, gamma), la) ps.
 
+Lemma invariant_iff_parse_table_for :
+  forall g ps tbl,
+    pairs_wf ps g
+    -> tbl_correct_wrt_pairs tbl ps
+       <-> parse_table_for tbl g.
+Proof.
+  intros g ps tbl Hwf.
+  split.
+  - intros Htc.
+    unfold tbl_correct_wrt_pairs in Htc.
+    split.
+    + unfold pt_sound.
+      intros x la gamma Hlk.
+      apply Hwf.
+      apply Htc; auto.
+    + unfold pt_complete.
+      intros la x gamma Hlk.
+      apply Htc.
+      apply Hwf; auto.
+  - intros Hpt.
+    destruct Hpt as [Hsou Hcom].
+    unfold tbl_correct_wrt_pairs.
+    intros x gamma la.
+    split.
+    + intros Hlk.
+      apply Hwf.
+      apply Hsou; auto.
+    + intros Hin.
+      apply Hcom.
+      apply Hwf; auto.
+Qed.
+
+Lemma addEntry_preserves_Some :
+  forall p o tbl,
+    addEntry p o = Some tbl
+    -> exists tbl',
+      o = Some tbl'.
+Proof.
+  intros p o tbl Hadd.
+  destruct p as ((x, gamma), la).
+  destruct o as [tbl' |] eqn:Ho.
+  - exists tbl'; auto.
+  - unfold addEntry in Hadd; inv Hadd.
+Qed.
+
+Lemma addEntry_preserves_invariant :
+  forall p ps tbl' tbl,
+    tbl_correct_wrt_pairs tbl' ps
+    -> addEntry p (Some tbl') = Some tbl
+    -> tbl_correct_wrt_pairs tbl (p :: ps).
+Proof.
+  intros p ps tbl' tbl Htc Hadd.
+  destruct p as ((x, gamma), la).
+  unfold tbl_correct_wrt_pairs.
+  intros x' gamma' la'.
+  split.
+  - intros Hlk.
+    simpl in Hadd.
+    unfold addEntry in Hadd.
+    destruct (NtMap.find x tbl') as [m |] eqn:Hnf.
+    + destruct (LaMap.find la m) as [gamma'' |] eqn:Hlf.
+      * destruct (list_eq_dec symbol_eq_dec gamma gamma'').
+
+Admitted.
+
+Lemma mkParseTable_satisfies_invariant :
+  forall ps tbl,
+         (* pairs_wf ps g *) (* this has to be global, not inductive *)
+    mkParseTable ps = Some tbl
+    -> tbl_correct_wrt_pairs tbl ps.
+Proof.
+  intros ps.
+  induction ps as [| p ps]; intros tbl Hmk; simpl in *.
+  - inv Hmk.
+    admit.
+  - pose proof Hmk as Hmk'.
+    apply addEntry_preserves_Some in Hmk.
+    destruct Hmk as [tbl' Hmk].
+    rewrite Hmk in Hmk'.
+    eapply addEntry_preserves_invariant; eauto.
+Admitted.
+
+(*
+  intros ps g Hwf.
+  induction ps as [| p ps]; intros tbl Hmk; simpl in *.
+  - inv Hmk.
+    unfold tbl_correct_wrt_pairs.
+    split.
+    + unfold tbl_sound_wrt_pairs.
+      intros x gamma la Hlk.
+      unfold pt_lookup in Hlk.
+      destruct (NtMap.find x empty_pt) eqn:Hnf.
+      * rewrite NtMapFacts.empty_o in Hnf; inv Hnf.
+      * inv Hlk.
+    + unfold tbl_complete_wrt_pairs.
+      intros x gamma la laSet Hin; inv Hin.
+  - pose proof Hmk as Hmk'.
+    apply addEntries_preserves_Some in Hmk.
+    destruct Hmk as [tbl' Hmk].
+    rewrite Hmk in Hmk'.
+    inv Hwf.
+    destruct p as ((x, gamma), laSet).
+    eapply addEntries_preserves_invariant; eauto.
+Qed.
+ *)
+
+Lemma mkParseTable_sound :
+  forall ps g tbl,
+    pairs_wf ps g
+    -> mkParseTable ps = Some tbl
+    -> parse_table_for tbl g.
+Proof.
+  intros ps g tbl Hwf Hmk.
+  eapply invariant_iff_parse_table_for; eauto.
+  eapply mkParseTable_satisfies_invariant; eauto.
+Qed.      
+      
+(*
 Definition tbl_sound_wrt_pairs tbl ps :=
   forall x gamma la,
     pt_lookup x la tbl = Some gamma
@@ -142,11 +259,63 @@ Proof.
       apply H; auto.
 Qed.
 
+Definition prod_la_pair := (production * LaSet.t)%type.
+
+Definition prod_la_pair_wf (g : grammar) (p : prod_la_pair) :=
+  match p with
+  | ((x, gamma), laSet) => lookahead_set_for laSet x gamma g
+  end.
+
+Definition prod_la_pairs_wf (ps : list prod_la_pair) (g : grammar) :=
+  Forall (prod_la_pair_wf g) ps.
+
+Definition empty_pt := NtMap.empty (LaMap.t (list symbol)).
+
+Definition singletonLaMap la gamma :=
+  LaMap.add la gamma (LaMap.empty (list symbol)).
+  
+Definition addEntry (x : nonterminal) (la : lookahead) (gamma : list symbol) (o : option parse_table) :=
+  match o with
+  | None => None
+  | Some tbl => 
+    match NtMap.find x tbl with
+    | None => Some (NtMap.add x (singletonLaMap la gamma) tbl)
+    | Some m =>
+      match LaMap.find la m with
+      | None => Some (NtMap.add x (LaMap.add la gamma m) tbl)
+      | Some gamma' =>
+        if list_eq_dec symbol_eq_dec gamma gamma' then Some tbl else None
+      end
+    end
+  end.
+
+Definition addEntries (p : prod_la_pair) (o : option parse_table) :=
+  match p with
+  | ((x, gamma), laSet) =>
+    fold_right (fun la o => addEntry x la gamma o) o (LaSet.elements laSet)
+  end.
+
+Definition mkParseTable (productions_with_la_sets : list prod_la_pair) :=
+  fold_right addEntries (Some empty_pt) productions_with_la_sets.
+
 Lemma addEntry_None_eq_None :
   forall x la gamma,
     addEntry x la gamma None = None.
 Proof.
   auto.
+Qed.
+
+Lemma addEntry_preserves_Some :
+  forall x la gamma o tbl,
+    addEntry x la gamma o = Some tbl
+    -> exists tbl',
+      o = Some tbl'.
+Proof.
+  intros x la gamma o tbl Hadd.
+  unfold addEntry in Hadd.
+  destruct o as [tbl' |] eqn:Ho.
+  - exists tbl'; auto.
+  - inv Hadd.
 Qed.
 
 Lemma addEntries_None_eq_None :
@@ -172,22 +341,113 @@ Proof.
   + rewrite addEntries_None_eq_None in H; inv H.
 Qed.
 
-Lemma addEntries_preserves_invariant :
-  forall tbl' tbl p ps,
-    tbl_correct_wrt_pairs tbl' ps
-    -> addEntries p (Some tbl') = Some tbl
-    -> tbl_correct_wrt_pairs tbl (p :: ps).
+Lemma empty_laSet_preserves_invariant :
+  forall tbl ps x gamma s,
+    tbl_correct_wrt_pairs tbl ps
+    -> LaSet.Empty s
+    -> tbl_correct_wrt_pairs tbl ((x, gamma, s) :: ps).
 Proof.
+  intros tbl ps x gamma s Htc Hem.
+  unfold tbl_correct_wrt_pairs.
+  split.
+  - unfold tbl_sound_wrt_pairs.
+    intros x' gamma' la Hlk.
+    destruct Htc as [Hsou Hcom].
+    apply Hsou in Hlk.
+    destruct Hlk as [s' [Hin Hlin]].
+    exists s'; split; auto.
+    right; auto.
+  - unfold tbl_complete_wrt_pairs.
+    intros x' gamma' la s' Hin Hlin.
+    inv Hin.
+    + inv H.
+      exfalso.
+      eapply Hem; eauto.
+    + destruct Htc as [_ Hcom].
+      eapply Hcom in H; eauto.
+Qed.
+
+Lemma addEntries_thang :
+  forall la laSet x gamma o tbl,
+    addEntries ((x, gamma), laSet) o = Some tbl
+    -> LaSet.In la laSet
+    -> pt_lookup x la tbl = Some gamma.
+Proof.
+  intros la laSet.
+  remember (LaSet.elements laSet) as elts.
+  generalize dependent laSet.
+  induction elts as [| e es].
+  - intros laSet Helts x gamma o tbl Hadd Hin.
+    admit.
+  - intros laSet Helts x gamma o tbl Hadd Hin.
+    pose proof Hadd as Hadd'.
+    unfold addEntries in Hadd.
+    rewrite <- Helts in Hadd; simpl in Hadd.
+    apply addEntry_preserves_Some in Hadd.
+    destruct Hadd as [tbl' Hfr].
+    unfold addEntries in IHes.
+    
+s    
+
+Lemma or_thing :
+  forall tbl' tbl ps x gamma laSet,
+    tbl_correct_wrt_pairs tbl' ps
+    -> addEntries ((x, gamma), laSet) (Some tbl') = Some tbl
+    -> (forall la,
+           LaSet.In la laSet -> pt_lookup x la tbl = Some gamma)
+    -> tbl_correct_wrt_pairs tbl ((x, gamma, laSet) :: ps).
+Proof.
+  intros.
+  unfold tbl_correct_wrt_pairs.
+  split.
+  - unfold tbl_sound_wrt_pairs.
+    intros x' gamma' la Hlk.
+    destruct H as [Hsou Hcom].
+    apply Hsou in Hlk.
+    destruct Hlk as [laSet' [Hin Hlin]].
+    exists laSet'; split; auto.
+    right; auto.
+  - unfold tbl_complete_wrt_pairs.
+    intros x' gamma' la laSet' Hin Hlin.
+    inv Hin.
+    + inv H1; auto.
+    + destruct H as [_ Hcom].
+      eapply Hcom in H1; eauto.
+Qed.
+            
+Lemma addEntries_preserves_invariant :
+  forall laSet x gamma
+         (tbl' tbl : parse_table)
+         (ps : list prod_la_pair),
+    tbl_correct_wrt_pairs tbl' ps
+    -> addEntries ((x, gamma), laSet) (Some tbl') = Some tbl
+    -> tbl_correct_wrt_pairs tbl (((x, gamma), laSet) :: ps).
+Proof.
+  intros.
+  intros laSet.
+  remember (LaSet.elements laSet) as elts.
+  generalize dependent laSet.
+  induction elts as [| e es].
+  - intros laSet Helts x gamma tbl' tbl ps Htc Hadd.
+    eapply empty_laSet_preserves_invariant.
+    + simpl in Hadd.
+      rewrite <- Helts in Hadd; simpl in Hadd.
+      inv Hadd; auto.
+    + apply LaSetEqProps.MP.elements_Empty; auto.
+  - intros laSet Helts x gamma tbl' tbl ps Htc Hadd.
+    
 Admitted.
+ *)
 
 Lemma mkParseTable_satisfies_invariant :
-  forall ps g tbl,
+  forall ps g,
     prod_la_pairs_wf ps g
-    -> mkParseTable ps = Some tbl
-    -> tbl_correct_wrt_pairs tbl ps.
+    -> forall tbl,
+      mkParseTable ps = Some tbl
+      -> tbl_correct_wrt_pairs tbl ps.
 Proof.
-  intros ps. 
-  induction ps as [| p ps]; intros g tbl Hwf Hmk; simpl in *.
+  intros ps g Hwf.
+  induction ps as [| p ps]; intros tbl Hmk; simpl in *.
   - inv Hmk.
     unfold tbl_correct_wrt_pairs.
     split.
@@ -204,6 +464,7 @@ Proof.
     destruct Hmk as [tbl' Hmk].
     rewrite Hmk in Hmk'.
     inv Hwf.
+    destruct p as ((x, gamma), laSet).
     eapply addEntries_preserves_invariant; eauto.
 Qed.
 
